functional big-step semantics for modLang expressions
a start on #89

compiler/backend/modLangScript.sml
@@ -32,6 +32,16 @@ val _ = Datatype`
   | Let (varN option) exp exp
   | Letrec ((varN # varN # exp) list) exp`;
 
+val exp_size_def = definition"exp_size_def";
+
+val exp6_size_APPEND = Q.store_thm("exp6_size_APPEND[simp]",
+  `modLang$exp6_size (e ++ e2) = exp6_size e + exp6_size e2`,
+  Induct_on`e`>>simp[exp_size_def])
+
+val exp6_size_REVERSE = Q.store_thm("exp6_size_REVERSE[simp]",
+  `modLang$exp6_size (REVERSE es) = exp6_size es`,
+  Induct_on`es`>>simp[exp_size_def])
+
 
 val _ = Datatype`
  dec =
